## Proof by induction

1. Base Case

2. Inductive hypothesis
  - k instances
  - k -> k + 1

#### Example Fibonacci

```
Claim:
  For all i >= 1, Fib number Fi < (5/3)^i

Base Case:
  i = 1
  F1 = (5/3)
  1 < (5/3) (This is true)
  F2 = 2 < (5/3)^2
  F2 = 2 < (25/9) (This is true)

Inductive hypothesis:
  assume Fi < (5/3)^i is true for all i <= k

We need to show:
  F(k+1) < (5/3)^(k+1)

  Fk+1 = Fk + Fk-1 (by Fibonacci definition)

induction step:
  F(k+1) < (5/3)^(k) + (5/3)^(k-1)
  F(k+1) < (3/5)(5/3)^(k) + (3/5)^(2) * (5/3)(k+1) -> (3/5)^2 because on the next term it is (5/3)^i
  F(k+1) < (3/5 + 9/25)*(5/3)^(k+1)
  F(k+1) < (24/25)(5/3)^(k+1)
  F(k+1) < (5/3)(k+1) -> (as 24/25 is less than 1)
```

#### Example 2

On pad
